template-coq/theories/Ast.v
@@ -3,7 +3,7 @@
 Require Import Coq.Strings.String.
 Require Import Coq.PArith.BinPos.
 Require Import List. Import ListNotations.
-From Template Require Export univ uGraph.
+From Template Require Export Universes.
 
 (** * AST of Coq kernel terms and kernel data structures
 
@@ -31,7 +31,7 @@ From Template Require Export univ uGraph.
     ** Environments of declarations
 
       The global environment [global_context]: a list of [global_decl] and
-    a universe graph [uGraph.t].  *)
+    a universe graph [constraints].  *)
 
 Require Export BasicAst.
 
@@ -88,7 +88,7 @@ Inductive wf : term -> Prop :=
 | wf_tProd na t b : wf t -> wf b -> wf (tProd na t b)
 | wf_tLambda na t b : wf t -> wf b -> wf (tLambda na t b)
 | wf_tLetIn na t b b' : wf t -> wf b -> wf b' -> wf (tLetIn na t b b')
-| wf_tApp t u : ~ isApp t = true -> u <> nil -> wf t -> Forall wf u -> wf (tApp t u)
+| wf_tApp t u : isApp t = false -> u <> nil -> wf t -> Forall wf u -> wf (tApp t u)
 | wf_tConst k u : wf (tConst k u)
 | wf_tInd i u : wf (tInd i u)
 | wf_tConstruct i k u : wf (tConstruct i k u)
@@ -233,7 +233,7 @@ Definition global_declarations := list global_decl.
 (** A context of global declarations + global universe constraints,
     i.e. a global environment *)
 
-Definition global_context : Type := global_declarations * uGraph.t.
+Definition global_context : Type := global_declarations * constraints.
 
 (** *** Programs
 
