template-coq/theories/utils.v
@@ -4,17 +4,36 @@ Require Import ssreflect.
 Set Asymmetric Patterns.
 Require Import Arith.
 
+(* Use \sum to input ∑ in Company Coq (it is not a sigma Σ). *)
+Notation "'∑' x .. y , p" := (sigT (fun x => .. (sigT (fun y => p%type)) ..))
+  (at level 200, x binder, right associativity,
+   format "'[' '∑'  '/  ' x  ..  y ,  '/  ' p ']'")
+  : type_scope.
+
+Notation "( x ; y )" := (@existT _ _ x y).
+Notation "( x ; y ; z )" := (x ; ( y ; z)).
+Notation "( x ; y ; z ; t )" := (x ; ( y ; (z ; t))).
+Notation "( x ; y ; z ; t ; u )" := (x ; ( y ; (z ; (t ; u)))).
+Notation "( x ; y ; z ; t ; u ; v )" := (x ; ( y ; (z ; (t ; (u ; v))))).
+Notation "x .1" := (@projT1 _ _ x) (at level 3, format "x '.1'").
+Notation "x .2" := (@projT2 _ _ x) (at level 3, format "x '.2'").
+
+Notation "x × y" := (prod x y )(at level 80, right associativity).
+
 Notation "#| l |" := (List.length l) (at level 0, l at level 99, format "#| l |").
+
+(* \circ *)
+Notation "g ∘ f" := (fun x => g (f x)).
 
 (** We cannot use ssrbool as it breaks extraction. *)
 Coercion is_true : bool >-> Sortclass.
 
 Definition pred (A : Type) := A -> bool.
 
-Lemma andb_and b b' : b && b' <-> b /\ b'.
+Lemma andb_and b b' : is_true (b && b') <-> is_true b /\ is_true b'.
 Proof. apply andb_true_iff. Qed.
 
-Lemma andP {b b'} : b && b' -> b /\ b'.
+Lemma andP {b b'} : is_true (b && b') -> is_true b /\ is_true b'.
 Proof. apply andb_and. Qed.
 
 Ltac toProp :=
@@ -557,7 +576,8 @@ Section Reverse_Induction.
 
 End Reverse_Induction.
 
-Lemma forallb_Forall {A} (p : pred A) l : Forall p l <-> forallb p l.
+Lemma forallb_Forall {A} (p : pred A) l
+  : Forall (is_true ∘ p) l <-> is_true (forallb p l).
 Proof.
   split.
   induction 1; rewrite /= // H IHForall //.
@@ -580,7 +600,7 @@ Qed.
 
 Lemma forallb2_All2 {A : Type} {p : A -> A -> bool}
       {l l' : list A} :
-  forallb2 p l l' -> All2 (fun x y => p x y) l l'.
+  is_true (forallb2 p l l') -> All2 (fun x y => is_true (p x y)) l l'.
 Proof.
   induction l in l' |- *; destruct l'; simpl; intros; try congruence.
   - constructor.
@@ -590,14 +610,15 @@ Qed.
 
 Lemma All2_forallb2 {A : Type} {p : A -> A -> bool}
       {l l' : list A} :
-  All2 (fun x y => p x y) l l' -> forallb2 p l l'.
+  All2 (fun x y => is_true (p x y)) l l' -> is_true (forallb2 p l l').
 Proof.
   induction 1; simpl; intros; try congruence.
   rewrite andb_and. intuition auto.
 Qed.
 
 Lemma forallb2_app {A} (p : A -> A -> bool) l l' q q' :
-  forallb2 p l l' && forallb2 p q q' -> forallb2 p (l ++ q) (l' ++ q').
+  is_true (forallb2 p l l' && forallb2 p q q')
+  -> is_true (forallb2 p (l ++ q) (l' ++ q')).
 Proof.
   induction l in l' |- *; destruct l'; simpl; try congruence.
   move=> /andP[/andP[pa pl] pq]. now rewrite pa IHl // pl pq.
@@ -660,12 +681,12 @@ Lemma All_Forall {A : Type} (P : A -> Prop) l :
   All P l -> Forall P l.
 Proof. induction 1; constructor; auto. Qed.
 
-Lemma forallb_All {A} (p : pred A) l : forallb p l -> All p l.
+Lemma forallb_All {A} (p : pred A) l : is_true (forallb p l) -> All (is_true ∘ p) l.
 Proof.
   move/forallb_Forall. apply Forall_All.
 Qed.
 
-Lemma All_forallb {A} (p : pred A) l : All p l -> forallb p l.
+Lemma All_forallb {A} (p : pred A) l : All (is_true ∘ p) l -> is_true (forallb p l).
 Proof.
   move/All_Forall. apply forallb_Forall.
 Qed.
@@ -854,8 +875,8 @@ Ltac All_map :=
 
 Lemma forall_forallb_map_spec {A B : Type} {P : A -> Prop} {p : A -> bool}
       {l : list A} {f g : A -> B} :
-    Forall P l -> forallb p l ->
-    (forall x : A, P x -> p x -> f x = g x) -> map f l = map g l.
+    Forall P l -> is_true (forallb p l) ->
+    (forall x : A, P x -> is_true (p x) -> f x = g x) -> map f l = map g l.
 Proof.
   induction 1; simpl; trivial.
   rewrite andb_and. intros [px pl] Hx.
@@ -864,16 +885,16 @@ Qed.
 
 Lemma forall_forallb_forallb_spec {A : Type} {P : A -> Prop} {p : A -> bool}
       {l : list A} {f : A -> bool} :
-    Forall P l -> forallb p l ->
-    (forall x : A, P x -> p x -> f x) -> forallb f l.
+    Forall P l -> is_true (forallb p l) ->
+    (forall x : A, P x -> is_true (p x) -> is_true (f x)) -> is_true (forallb f l).
 Proof.
   induction 1; simpl; trivial.
   rewrite !andb_and. intros [px pl] Hx. eauto.
 Qed.
 
 Lemma on_snd_test_spec {A B C} (P : B -> Prop) (p : B -> bool) (f g : B -> C) (x : A * B) :
-  P (snd x) -> (forall x, P x -> p x -> f x = g x) ->
-  test_snd p x ->
+  P (snd x) -> (forall x, P x -> is_true (p x) -> f x = g x) ->
+  is_true (test_snd p x) ->
   on_snd f x = on_snd g x.
 Proof.
   intros. destruct x. unfold on_snd. simpl.
@@ -1278,16 +1299,16 @@ Qed.
 
 Lemma All_forallb' {A} P (l : list A) (p : pred A) :
   All P l ->
-  (forall x, P x -> p x) ->
-  forallb p l.
+  (forall x, P x -> is_true (p x)) ->
+  is_true (forallb p l).
 Proof.
   induction 1 in p |- *; unfold compose; simpl; rewrite ?andb_and;
     intuition auto.
 Qed.
 
 Lemma forallb_Forall' {A} (P : A -> Prop) (l : list A) p :
-  forallb p l ->
-  (forall x, p x -> P x) ->
+  is_true (forallb p l) ->
+  (forall x, is_true (p x) -> P x) ->
   Forall P l.
 Proof.
   induction l in p |- *; unfold compose; simpl. constructor.
@@ -1295,8 +1316,8 @@ Proof.
 Qed.
 
 Lemma forallb_skipn {A} (p : A -> bool) n l :
-  forallb p l ->
-  forallb p (skipn n l).
+  is_true (forallb p l) ->
+  is_true (forallb p (skipn n l)).
 Proof.
   induction l in n |- *; destruct n; simpl; try congruence.
   intros. apply IHl. rewrite -> andb_and in H; intuition.
@@ -1318,7 +1339,7 @@ Proof.
   induction 1; simpl; intuition (f_equal; auto).
 Qed.
 
-Lemma forallb2_length {A} (p : A -> A -> bool) l l' : forallb2 p l l' -> length l = length l'.
+Lemma forallb2_length {A} (p : A -> A -> bool) l l' : is_true (forallb2 p l l') -> length l = length l'.
 Proof.
   induction l in l' |- *; destruct l'; simpl; try congruence.
   rewrite !andb_and. intros [Hp Hl]. erewrite IHl; eauto.
@@ -1370,8 +1391,8 @@ Qed.
 
 Lemma Forall_forallb {A} P (l : list A) (p : pred A) :
   Forall P l ->
-  (forall x, P x -> p x) ->
-  forallb p l.
+  (forall x, P x -> is_true (p x)) ->
+  is_true (forallb p l).
 Proof.
   induction 1 in p |- *; unfold compose; simpl; rewrite ?andb_and;
     intuition auto.
@@ -1388,3 +1409,31 @@ Lemma Forall2_non_nil {A B} (P : A -> B -> Prop) (l : list A) (l' : list B) :
 Proof.
   induction 1; congruence.
 Qed.
+
+(* Sorted lists without duplicates *)
+Class ComparableType A := { compare : A -> A -> comparison }.
+Arguments compare {A} {_} _ _.
+
+Fixpoint insert {A} `{ComparableType A} (x : A) (l : list A) :=
+  match l with
+  | [] => [x]
+  | y :: l' =>  match compare x y with
+               | Eq => l
+               | Lt => x :: l
+               | Gt => y :: (insert x l')
+               end
+  end.
+
+Definition list_union {A} `{ComparableType A} (l l' : list A) : list A
+  := fold_left (fun l' x => insert x l') l l'.
+
+Definition compare_bool b1 b2 :=
+  match b1, b2 with
+  | false, true => Lt
+  | true, false => Gt
+  | _, _ => Eq
+  end.
+
+Definition bool_lt' b1 b2 := match compare_bool b1 b2 with Lt => true | _ => false end.
+
+Definition non_empty_list (A : Set) := {l : list A & [] <> l}.
